

$$\begin{bmatrix}
f-g.\sqrt{\frac{N-n}{N-1}}.\sqrt{\frac{p.(1-p)}{n}}; f+g.\sqrt{\frac{N-n}{N-1}}.\sqrt{\frac{p.(1-p)}{n}}
\end{bmatrix}$$

f = 180/200

ME = $1.96.\sqrt{\frac{N-n}{N-1}}.\sqrt{\frac{p.(1-p)}{n}}$ = 0,0513
$$
g.\sqrt{\frac{2300}{2499}}.\sqrt{\frac{p.(1-p)}{n}} = 0,0513\\
g.\ 0,9593581954926447\ .\sqrt{\frac{p.(1-p)}{n}} = 0,0513\\
g.\sqrt{\frac{0,9.(1-0,9)}{200}} =0,0534732493463056\\
g.=\frac{0,0534732493463056}{\sqrt{\frac{0,9.(1-0,9)}{200}}}\\
a=2,52\\

g=1-\frac{\alpha}{2}\\
$$


